src/Init/Data/String/Defs.lean
@@ -399,7 +399,7 @@ achieved by tracking the bounds by hand, the slice API is much more convenient.
 string. For this reason, it should be preferred over `Substring.Raw`.
 -/
 structure Slice where
-  /-- The underlying strings. -/
+  /-- The underlying string. -/
   str : String
   /-- The byte position of the start of the string slice. -/
   startInclusive : str.Pos
@@ -440,6 +440,18 @@ def Slice.utf8ByteSize (s : Slice) : Nat :=
 
 theorem Slice.utf8ByteSize_eq {s : Slice} :
     s.utf8ByteSize = s.endExclusive.offset.byteIdx - s.startInclusive.offset.byteIdx := (rfl)
+
+/--
+Checks whether a slice is empty.
+
+Empty slices have {name}`utf8ByteSize` {lean}`0`.
+
+Examples:
+ * {lean}`"".toSlice.isEmpty = true`
+ * {lean}`" ".toSlice.isEmpty = false`
+-/
+@[inline]
+def Slice.isEmpty (s : Slice) : Bool := s.utf8ByteSize == 0
 
 instance : HAdd Pos.Raw Slice Pos.Raw where
   hAdd p s := { byteIdx := p.byteIdx + s.utf8ByteSize }
@@ -629,18 +641,6 @@ def Slice.Pos.byte {s : Slice} (pos : s.Pos) (h : pos ≠ s.endPos) : UInt8 :=
 
 theorem push_eq_append (c : Char) : String.push s c = s ++ singleton c := by
   simp
-
-/--
-Checks whether a slice is empty.
-
-Empty slices have {name}`utf8ByteSize` {lean}`0`.
-
-Examples:
- * {lean}`"".toSlice.isEmpty = true`
- * {lean}`" ".toSlice.isEmpty = false`
--/
-@[inline]
-def Slice.isEmpty (s : Slice) : Bool := s.utf8ByteSize == 0
 
 @[simp]
 theorem Slice.Pos.le_refl {s : Slice} (p : s.Pos) : p ≤ p := by
