src/Init/Data/String/Lemmas/Split2.lean
@@ -1,0 +1,1050 @@
+/-
+Copyright (c) 2026 Lean FRO, LLC. All rights reserved.
+Released under Apache 2.0 license as described in the file LICENSE.
+Authors: Markus Himmel
+-/
+module
+
+prelude
+public import Init.Data.String.Pattern.Basic
+public import Init.Data.String.Subslice
+public import Init.Data.String.Lemmas.Splits
+public import Init.Data.String.Slice
+import all Init.Data.String.Slice
+import all Init.Data.String.Pattern.Basic
+import all Init.Data.String.Pattern.String
+import all Init.Data.String.Defs
+import Init.Data.String.Lemmas.IsEmpty
+import Init.Data.String.Lemmas.Basic
+import Init.Data.String.Termination
+import Init.Data.ByteArray.Lemmas
+import Init.Data.String.Lemmas.Order
+import Init.Data.String.OrderInstances
+import Init.Data.Iterators.Lemmas.Consumers.Collect
+import Init.Data.Vector.Lemmas
+import Init.Grind
+import Init.Data.Iterators.Lemmas.Basic
+public import Init.Data.String.Lemmas.Pattern
+
+public section
+
+namespace String
+
+@[simp]
+theorem Pos.Raw.isValidForSlice_zero {s : Slice} : (0 : Pos.Raw).IsValidForSlice s where
+  le_rawEndPos := by simp [Pos.Raw.le_iff]
+  isValid_offsetBy := by simpa using s.startInclusive.isValid
+
+end String
+
+namespace String.Slice
+
+@[simp]
+theorem Pos.isValidForSlice_offset {s : Slice} {p : s.Pos} : p.offset.IsValidForSlice s :=
+  p.isValidForSlice
+
+@[simp]
+theorem pos_rawEndPos {s : Slice} : s.pos s.rawEndPos Pos.Raw.isValidForSlice_rawEndPos = s.endPos := by
+  simp [Pos.ext_iff]
+
+theorem Slice.splits_next_startPos {s : Slice} {h : s.startPos ≠ s.endPos} :
+    (s.startPos.next h).Splits (singleton (s.startPos.get h)) (s.sliceFrom (s.startPos.next h)).copy := by
+  rw [← String.empty_append (s := singleton (s.startPos.get h))]
+  apply Slice.Pos.Splits.next
+  have := Slice.Pos.splits_next_right s.startPos h
+  rwa [copy_sliceTo_startPos] at this
+
+@[simp]
+theorem copy_pos {s : Slice} {p : Pos.Raw} {h : Pos.Raw.IsValidForSlice s p} :
+    (s.pos p h).copy = s.copy.pos p (Pos.Raw.isValid_copy_iff.2 h) := by
+  simp [String.Pos.ext_iff]
+
+@[simp]
+theorem _root_.String.cast_pos {s t : String} {p : Pos.Raw} {h : Pos.Raw.IsValid s p} {h' : s = t} :
+    (s.pos p h).cast h' = t.pos p (h' ▸ h) := by
+  simp [String.Pos.ext_iff]
+
+theorem Pos.ne_of_lt {s : Slice} {p q : s.Pos} : p < q → p ≠ q := by
+  simpa [Pos.ext_iff, Pos.Raw.ext_iff, Pos.lt_iff, Pos.Raw.lt_iff] using Nat.ne_of_lt
+
+theorem Pos.Splits.copy_sliceTo_eq {s : Slice} {p : s.Pos} (h : p.Splits t₁ t₂) :
+    (s.sliceTo p).copy = t₁ :=
+  p.splits.eq_left h
+
+theorem Pos.Splits.copy_sliceFrom_eq {s : Slice} {p : s.Pos} (h : p.Splits t₁ t₂) :
+    (s.sliceFrom p).copy = t₂ :=
+  p.splits.eq_right h
+
+theorem _root_.String.Pos.splits_append_rawEndPos {s t : String} :
+    ((s ++ t).pos s.rawEndPos ((Pos.Raw.isValid_rawEndPos).append_right t)).Splits s t where
+  eq_append := rfl
+  offset_eq_rawEndPos := rfl
+
+theorem pos!_eq_pos {s : Slice} {p : Pos.Raw} (h : p.IsValidForSlice s) :
+    s.pos! p = s.pos p h := by
+  simp [Slice.pos!, h]
+
+theorem _root_.String.pos!_eq_pos {s : String} {p : Pos.Raw} (h : p.IsValid s) :
+    s.pos! p = s.pos p h := by
+  rw [String.pos!, Slice.pos!_eq_pos h.toSlice, String.pos]
+
+section BEq
+
+@[simp]
+theorem beq_eq_true_iff {s t : Slice} : s == t ↔ s.copy = t.copy := by
+  simp only [BEq.beq, beq]
+  split <;> rename_i h
+  · rw [Pattern.Internal.memcmpSlice_eq_true_iff]
+    simp only [offset_startPos, Pos.Raw.byteIdx_zero, Pos.Raw.offsetBy_zero, byteIdx_rawEndPos]
+    rw (occs := [2]) [h]
+    rw [utf8ByteSize_eq_size_toByteArray_copy, ByteArray.extract_zero_size,
+      utf8ByteSize_eq_size_toByteArray_copy, ByteArray.extract_zero_size, String.toByteArray_inj]
+  · simpa using ne_of_apply_ne String.utf8ByteSize (by simpa)
+
+@[simp]
+theorem beq_eq_false_iff {s t : Slice} : (s == t) = false ↔ s.copy ≠ t.copy := by
+  simp [← Bool.not_eq_true]
+
+theorem beq_eq_decide {s t : Slice} : (s == t) = decide (s.copy = t.copy) := by
+  cases h : s == t <;> simp_all
+
+end BEq
+
+namespace Pattern
+
+
+/-
+Is there a correctness statement for searching beyond what I already have???
+-/
+
+@[ext]
+structure SplitFrom {s : Slice} (startPos : s.Pos) where
+  l : List s.Subslice
+  any_head? : l.head?.any (·.startInclusive = startPos)
+
+def SplitFrom.at {s : Slice} (pos : s.Pos) : SplitFrom pos where
+  l := [s.subslice pos pos (Slice.Pos.le_refl _)]
+  any_head? := by simp
+
+@[simp]
+theorem SplitFrom.l_at {s : Slice} (pos : s.Pos) :
+    (SplitFrom.at pos).l = [s.subslice pos pos (Slice.Pos.le_refl _)] := (rfl)
+
+def SplitFrom.append {s : Slice} {p₁ p₂ : s.Pos} (l₁ : SplitFrom p₁) (l₂ : SplitFrom p₂) :
+    SplitFrom p₁ where
+  l := l₁.l ++ l₂.l
+  any_head? := by simpa using Option.any_or_of_any_left l₁.any_head?
+
+@[simp]
+theorem SplitFrom.l_append {s : Slice} {p₁ p₂ : s.Pos} {l₁ : SplitFrom p₁} {l₂ : SplitFrom p₂} :
+    (l₁.append l₂).l = l₁.l ++ l₂.l :=
+  (rfl)
+
+def SplitFrom.extend {s : Slice} (p₁ : s.Pos) {p₂ : s.Pos} (h : p₁ ≤ p₂) (l : SplitFrom p₂) :
+    SplitFrom p₁ where
+  l :=
+    match l.l, l.any_head? with
+    | st :: sts, h => st.extendLeft p₁ (by simp_all) :: sts
+  any_head? := by split; simp
+
+@[simp]
+theorem SplitFrom.l_extend {s : Slice} {p₁ p₂ : s.Pos} (h : p₁ ≤ p₂) {l : SplitFrom p₂} :
+    (l.extend p₁ h).l = match l.l, l.any_head? with | st :: sts, h => st.extendLeft p₁ (by simp_all) :: sts := (rfl)
+
+@[simp]
+theorem SplitFrom.extend_self {s : Slice} {p₁ : s.Pos} (l : SplitFrom p₁) :
+    l.extend p₁ (Slice.Pos.le_refl _) = l := by
+  rcases l with ⟨l, h⟩
+  match l, h with
+  | st :: sts, h =>
+    simp at h
+    simp [SplitFrom.extend, ← h]
+
+@[simp]
+theorem SplitFrom.extend_extend {s : Slice} {p₀ p₁ p₂ : s.Pos} {h : p₀ ≤ p₁} {h' : p₁ ≤ p₂}
+    {l : SplitFrom p₂} : (l.extend p₁ h').extend p₀ h = l.extend p₀ (Slice.Pos.le_trans h h') := by
+  rcases l with ⟨l, h⟩
+  match l, h with
+  | st :: sts, h => simp [SplitFrom.extend]
+
+open Classical in
+noncomputable def dropPrefixAt?Model {ρ : Type} (pat : ρ) [ForwardPatternModel pat] {s : Slice}
+    (start : s.Pos) : Option s.Pos :=
+  if h : ∃ pos, IsLongestMatchAt pat start pos then some h.choose else none
+
+theorem dropPrefixAt?Model_eq_none_of_not_matchesAt {ρ : Type} {pat : ρ} [ForwardPatternModel pat]
+    {s : Slice} {start : s.Pos} (h : ¬ MatchesAt pat start) :
+    dropPrefixAt?Model pat start = none := by
+  rw [dropPrefixAt?Model, dif_neg]
+  simp only [not_exists]
+  exact fun p hp => h ⟨⟨_, hp⟩⟩
+
+theorem isLongestMatchAt_of_dropPrefixAt?Model_eq_some {ρ : Type} {pat : ρ} [ForwardPatternModel pat]
+    {s : Slice} {pos pos' : s.Pos} (h : dropPrefixAt?Model pat pos = some pos') :
+    IsLongestMatchAt pat pos pos' := by
+  simp [dropPrefixAt?Model] at h
+  obtain ⟨h, rfl⟩ := h
+  exact Exists.choose_spec _
+
+theorem dropPrefixAt?Model_eq_some_of_isLongestMatchAt {ρ : Type} {pat : ρ} [ForwardPatternModel pat]
+    {s : Slice} {pos pos' : s.Pos} (h : IsLongestMatchAt pat pos pos') :
+    dropPrefixAt?Model pat pos = some pos' := by
+  have h₀ : ∃ p, IsLongestMatchAt pat pos p := ⟨_, h⟩
+  have : ∃ p, dropPrefixAt?Model pat pos = some p ∧ IsLongestMatchAt pat pos p := by
+    simpa [dropPrefixAt?Model, h₀] using Exists.choose_spec _
+  obtain ⟨p, h₁, h₂⟩ := this
+  rw [h₁, Option.some.injEq, h₂.eq h]
+
+theorem lt_of_dropPrefixAt?Model_eq_some {ρ : Type} {pat : ρ} [ForwardPatternModel pat]
+    {s : Slice} {pos pos' : s.Pos} (h : dropPrefixAt?Model pat pos = some pos') : pos < pos' :=
+  isLongestMatchAt_of_dropPrefixAt?Model_eq_some h |>.lt
+
+noncomputable def splitModel {ρ : Type} (pat : ρ) [ForwardPatternModel pat] {s : Slice}
+    (start : s.Pos) : SplitFrom start :=
+  if h : start = s.endPos then
+    SplitFrom.at start
+  else
+    match hd : dropPrefixAt?Model pat start with
+    | some pos =>
+      have : start < pos := lt_of_dropPrefixAt?Model_eq_some hd
+      (SplitFrom.at start).append (splitModel pat pos)
+    | none => SplitFrom.extend start (by simp) (splitModel pat (start.next h))
+termination_by start
+
+theorem splitModel_eq_of_isLongestMatchAt {ρ : Type} {pat : ρ} [ForwardPatternModel pat] {s : Slice}
+    {start stop : s.Pos} (h : IsLongestMatchAt pat start stop) :
+    splitModel pat start = (SplitFrom.at start).append (splitModel pat stop) := by
+  rw [splitModel, dif_neg (Slice.Pos.ne_endPos_of_lt h.lt)]
+  split
+  · rename_i p heq
+    simp [dropPrefixAt?Model_eq_some_of_isLongestMatchAt h] at heq
+    congr <;> exact heq.symm
+  · rename_i heq
+    simp [dropPrefixAt?Model_eq_some_of_isLongestMatchAt h] at heq
+
+theorem splitModel_eq_of_not_matchesAt {ρ : Type} {pat : ρ} [ForwardPatternModel pat] {s : Slice}
+    {start stop : s.Pos} (h₀ : start ≤ stop) (h : ∀ p, start ≤ p → p < stop → ¬ MatchesAt pat p) :
+    splitModel pat start = (SplitFrom.extend start h₀ (splitModel pat stop)) := by
+  induction start using WellFounded.induction Slice.Pos.wellFounded_gt with | h start ih
+  by_cases h' : start < stop
+  · rw [splitModel, dif_neg (Slice.Pos.ne_endPos_of_lt h')]
+    have : ¬ MatchesAt pat start := h start (Slice.Pos.le_refl _) h'
+    split
+    · rename_i heq
+      simp [dropPrefixAt?Model_eq_none_of_not_matchesAt this] at heq
+    · rw [ih, SplitFrom.extend_extend]
+      · simp
+      · simp [h']
+      · refine fun p hp₁ hp₂ => h p (Std.le_of_lt (by simpa using hp₁)) hp₂
+  · obtain rfl : start = stop := Std.le_antisymm h₀ (Std.not_lt.1 h')
+    rw [SplitFrom.extend_self]
+
+def splitOnLists {s : Slice} (currPos : s.Pos) (l : List (SearchStep s)) : List s.Subslice :=
+  match l with
+  | [] => [s.subsliceFrom currPos]
+  | .rejected .. :: l => splitOnLists currPos l
+  | .matched p q :: l => s.subslice! currPos p :: splitOnLists q l
+
+theorem IsValidSearchFrom.splitOnLists_eq_splitModel {ρ : Type} (pat : ρ) [ForwardPatternModel pat]
+    (l : List (SearchStep s)) (pos pos' : s.Pos) (h₀ : pos ≤ pos')
+    (h' : ∀ p, pos ≤ p → p < pos' → ¬ MatchesAt pat p)
+    (h : IsValidSearchFrom pat pos' l) :
+    splitOnLists pos l = ((splitModel pat pos').extend pos h₀).l := by
+  induction h generalizing pos with
+  | endPos =>
+    simp [splitOnLists, splitModel]
+    split
+    simp_all only [SplitFrom.l_at, List.cons.injEq, List.nil_eq, List.head?_cons, Option.any_some,
+      decide_eq_true_eq, heq_eq_eq, and_true]
+    rename_i h
+    simp only [← h.1]
+    ext <;> simp
+  | matched h valid ih =>
+    rename_i l startPos endPos
+    simp only [splitOnLists]
+    rw [subslice!_eq_subslice h₀, splitModel_eq_of_isLongestMatchAt h]
+    simp [SplitFrom.at, SplitFrom.append]
+    refine ⟨?_, ?_⟩
+    · ext <;> simp
+    · rw [ih endPos (Slice.Pos.le_refl _), SplitFrom.extend_self]
+      intro p hp₁ hp₂
+      exact False.elim (Std.lt_irrefl (Std.lt_of_le_of_lt hp₁ hp₂))
+  | mismatched h rej valid ih =>
+    simp only [splitOnLists]
+    rename_i l startPos endPos
+    rw [splitModel_eq_of_not_matchesAt (Std.le_of_lt h) rej,
+      SplitFrom.extend_extend]
+    rw [ih]
+    intro p hp₁ hp₂
+    by_cases hp : p < startPos
+    · exact h' p hp₁ hp
+    · exact rej _ (Std.not_lt.1 hp) hp₂
+
+theorem toList_eq_splitOnLists' {ρ : Type} {pat : ρ} {σ : Slice → Type} [ToForwardSearcher pat σ]
+    [∀ s, Std.Iterator (σ s) Id (SearchStep s)] [∀ s, Std.Iterators.Finite (σ s) Id] {s : Slice}
+    (it : Std.Iter (α := σ s) (SearchStep s)) (currPos : s.Pos) :
+    (Std.Iter.mk (α := SplitIterator pat s) (.operating currPos it)).toList =
+      splitOnLists currPos it.toList := by
+  induction it using Std.Iter.inductSteps generalizing currPos with | step it ihy ihs
+  rw [Std.Iter.toList_eq_match_step, Std.Iter.step_eq]
+  conv => rhs; rw [Std.Iter.toList_eq_match_step]
+  simp [Std.Iter.toIterM]
+  cases it.step using Std.PlausibleIterStep.casesOn with
+  | yield it out h =>
+    match out with
+    | .matched startPos endPos =>
+      simp [splitOnLists]
+      rw [← ihy h]
+    | .rejected startPos endPos =>
+      simp [splitOnLists]
+      rw [← ihy h]
+  | skip it h =>
+    simp
+    rw [← ihs h]
+  | done =>
+    simp [splitOnLists]
+    have : (Std.Iter.mk (α := SplitIterator pat s) SplitIterator.atEnd).toList = [] := by
+      rw [Std.Iter.toList_eq_match_step, Std.Iter.step_eq]
+      simp [Std.Iter.toIterM]
+    rw [← this]
+
+theorem toList_eq_splitOnLists {ρ : Type} {pat : ρ} {σ : Slice → Type} [ToForwardSearcher pat σ]
+    [∀ s, Std.Iterator (σ s) Id (SearchStep s)] [∀ s, Std.Iterators.Finite (σ s) Id] (s : Slice) :
+    (s.splitToSubslice pat).toList = splitOnLists s.startPos (ToForwardSearcher.toSearcher pat s).toList := by
+  rw [splitToSubslice, toList_eq_splitOnLists']
+
+theorem toList_eq_splitModel {ρ : Type} (pat : ρ) [ForwardPatternModel pat]
+    {σ : Slice → Type} [ToForwardSearcher pat σ] [∀ s, Std.Iterator (σ s) Id (SearchStep s)]
+    [∀ s, Std.Iterators.Finite (σ s) Id] [LawfulToForwardSearcherModel pat] (s : Slice) :
+    (s.splitToSubslice pat).toList = (splitModel pat s.startPos).l := by
+  rw [toList_eq_splitOnLists, IsValidSearchFrom.splitOnLists_eq_splitModel pat _
+    s.startPos s.startPos (Std.le_refl _) _ (LawfulToForwardSearcherModel.isValidSearchFrom_toList _),
+    SplitFrom.extend_self]
+  exact fun p hp₁ hp₂ => False.elim (Std.lt_irrefl (Std.lt_of_le_of_lt hp₁ hp₂))
+
+namespace ForwardSliceSearcher
+
+instance {pat : Slice} : ForwardPatternModel pat where
+  Matches s := s ≠ "" ∧ s = pat.copy
+  not_matches_empty := by simp
+
+instance {pat : Slice} : NoPrefixForwardPatternModel pat :=
+  .of_length_eq (by simp +contextual [ForwardPatternModel.Matches])
+
+theorem isMatch_iff {pat s : Slice} {pos : s.Pos} (h : pat.isEmpty = false) :
+    IsMatch pat pos ↔ (s.sliceTo pos).copy = pat.copy := by
+  simp only [Pattern.isMatch_iff, ForwardPatternModel.Matches, ne_eq, copy_eq_empty_iff,
+    Bool.not_eq_true, and_iff_right_iff_imp]
+  intro h'
+  rw [← isEmpty_copy (s := s.sliceTo pos), h', isEmpty_copy, h]
+
+theorem isLongestMatch_iff {pat s : Slice} {pos : s.Pos} (h : pat.isEmpty = false) :
+    IsLongestMatch pat pos ↔ (s.sliceTo pos).copy = pat.copy := by
+  rw [isLongestMatch_iff_isMatch, isMatch_iff h]
+
+theorem isLongestMatchAt_iff_extract {pat s : Slice} {pos₁ pos₂ : s.Pos} (h : pat.isEmpty = false) :
+    IsLongestMatchAt pat pos₁ pos₂ ↔ s.copy.toByteArray.extract pos₁.offset.byteIdx pos₂.offset.byteIdx = pat.copy.toByteArray := by
+
+  have heq (h₁ : pos₁ ≤ pos₂) :
+      min (s.startInclusive.offset.byteIdx + pos₂.offset.byteIdx) s.endExclusive.offset.byteIdx =
+        s.startInclusive.offset.byteIdx + pos₁.offset.byteIdx + (pos₂.offset.byteIdx - pos₁.offset.byteIdx) := by
+    have := pos₂.str_le_endExclusive
+    simp only [Pos.le_iff, Pos.Raw.le_iff, String.Pos.le_iff, Pos.offset_str,
+      Pos.Raw.byteIdx_offsetBy] at h₁ this
+    omega
+  refine ⟨fun ⟨h₁, h₂⟩ => ?_, fun h' => ?_⟩
+  · rw [isLongestMatch_iff h] at h₂
+    rw [← h₂]
+    simp [toByteArray_copy, ByteArray.extract_extract, heq h₁]
+  · have h₁ : pos₁ ≤ pos₂ := by
+      have := congrArg ByteArray.size h'
+      simp at this
+      simp [isEmpty_eq] at h
+      simp [Pos.le_iff, Pos.Raw.le_iff]
+      omega
+    refine ⟨h₁, ?_⟩
+    rw [isLongestMatch_iff h]
+    simp [← toByteArray_inj, ← h']
+    simp [toByteArray_copy, ByteArray.extract_extract, heq h₁]
+
+theorem size_le_of_matchesAt {pat s : Slice} (hpat : pat.isEmpty = false) {pos : s.Pos} :
+    MatchesAt pat pos → pos.offset.byteIdx + pat.copy.toByteArray.size ≤ s.copy.toByteArray.size := by
+  rintro ⟨⟨endPos, hend⟩⟩
+  rw [isLongestMatchAt_iff_extract hpat] at hend
+  have h₁ := congrArg ByteArray.size hend
+  have h₂ := pos.str_le_endExclusive
+  simp [String.Pos.le_iff, Pos.Raw.le_iff, utf8ByteSize_eq] at ⊢ h₁ h₂
+  omega
+
+theorem not_matchesAt_of_getUTF8Byte_ne {pat s : Slice} (hpat : pat.isEmpty = false) {pos : s.Pos} (off : Pos.Raw)
+    {hoff₁ hoff₂}
+    (h : s.getUTF8Byte (off.offsetBy pos.offset) hoff₁ ≠ pat.getUTF8Byte off hoff₂) :
+    ¬ MatchesAt pat pos := by
+  rintro ⟨⟨endPos, hend⟩⟩
+  rw [isLongestMatchAt_iff_extract hpat] at hend
+  have := congrArg (·[off.byteIdx]?) hend
+  simp at this
+  rw [getElem?_pos, getElem?_pos, Option.some.injEq, ByteArray.getElem_extract] at this
+  · simp [getUTF8Byte_eq_getUTF8Byte_copy, String.getUTF8Byte, this] at h
+  · simpa [Pos.Raw.lt_iff] using hoff₂
+  · simp only [ByteArray.size_extract, size_toByteArray, utf8ByteSize_copy]
+    have ht₀ := endPos.isValidForSlice.le_utf8ByteSize
+    rw [Nat.min_eq_left (by omega)]
+    have : endPos.offset.byteIdx - pos.offset.byteIdx = pat.endExclusive.offset.byteIdx - pat.startInclusive.offset.byteIdx := by
+      have := congrArg ByteArray.size hend
+      simp only [ByteArray.size_extract, size_toByteArray, utf8ByteSize_copy] at this
+      rwa [Nat.min_eq_left (by omega)] at this
+    simp [Pos.Raw.lt_iff, utf8ByteSize_eq] at hoff₂
+    omega
+
+theorem getElem_eq_of_matchesAt {pat s : Slice} (hpat : pat.isEmpty = false) {pos : s.Pos}
+    (h : MatchesAt pat pos) (j : Nat) (hj : j < pat.copy.toByteArray.size) :
+    pat.copy.toByteArray[j]'hj = s.copy.toByteArray[pos.offset.byteIdx + j]'(by have := size_le_of_matchesAt hpat h; omega) := by
+  rcases h with ⟨⟨endPos, hend⟩⟩
+  rw [isLongestMatchAt_iff_extract hpat] at hend
+  simp only [← hend]
+  simp [ByteArray.getElem_extract]
+
+theorem le_of_matchesAt {pat s : Slice} (hpat : pat.isEmpty = false) {pos : s.Pos}
+    (h : MatchesAt pat pos) : pos.offset.byteIdx + pat.utf8ByteSize ≤ s.utf8ByteSize := by
+  obtain ⟨⟨endPos, hend⟩⟩ := h
+  rw [isLongestMatchAt_iff_extract hpat] at hend
+  replace hend := congrArg ByteArray.size hend
+  simp [utf8ByteSize_eq] at ⊢ hend
+  have := endPos.str_le_endExclusive
+  simp [String.Pos.le_iff, Pos.Raw.le_iff] at this
+  rw [Nat.min_eq_left (by omega)] at hend
+  rw [← hend]
+  simp [Slice.isEmpty_eq, utf8ByteSize_eq] at hpat
+  omega
+
+theorem startsWith_iff {pat s : Slice} : startsWith pat s ↔ ∃ t, s.copy = pat.copy ++ t := by
+  fun_cases startsWith with
+  | case1 h hs hp =>
+    rw [Internal.memcmpSlice_eq_true_iff]
+    refine ⟨fun h => ?_, fun ⟨t, ht⟩ => ?_⟩
+    · simp at h
+      rw (occs := [2]) [utf8ByteSize_eq_size_toByteArray_copy] at h
+      rw [ByteArray.extract_zero_size] at h
+      refine ⟨⟨s.copy.toByteArray.extract pat.utf8ByteSize s.utf8ByteSize, ?_⟩, ?_⟩
+      · rw [utf8ByteSize_eq_size_toByteArray_copy (s := s)]
+        apply Pos.Raw.IsValid.isValidUTF8_extract_utf8ByteSize
+        rw [Pos.Raw.isValid_iff_isValidUTF8_extract_zero]
+        simp only
+        rw [← pat.utf8ByteSize_eq, h]
+        exact ⟨by simpa [Pos.Raw.le_iff], pat.copy.isValidUTF8⟩
+      · rw [← toByteArray_inj, toByteArray_append]
+        simp only [← h]
+        rw [ByteArray.extract_append_extract, Nat.min_eq_left (Nat.zero_le _), Nat.max_eq_right ‹_›,
+          utf8ByteSize_eq_size_toByteArray_copy, ByteArray.extract_zero_size]
+    · simp [ht]
+      rw [ByteArray.extract_append_eq_left utf8ByteSize_eq_size_toByteArray_copy,
+        utf8ByteSize_eq_size_toByteArray_copy, ByteArray.extract_zero_size]
+  | case2 =>
+    simp only [Bool.false_eq_true, false_iff, not_exists]
+    intro t
+    apply ne_of_apply_ne String.utf8ByteSize
+    simp [utf8ByteSize_eq] at *
+    omega
+
+theorem dropPrefix?_eq_some_iff {pat s : Slice} {pos : s.Pos} :
+    dropPrefix? pat s = some pos ↔ (s.sliceTo pos).copy = pat.copy := by
+  fun_cases dropPrefix? with
+  | case1 h =>
+    obtain ⟨t, ht⟩ := startsWith_iff.1 h
+    have hval : pat.rawEndPos.IsValidForSlice s := by
+      rw [← Pos.Raw.isValid_copy_iff, ht, ← Slice.rawEndPos_copy]
+      exact Pos.Raw.isValid_rawEndPos.append_right _
+    refine ⟨?_, ?_⟩
+    · have hsplit : (s.pos pat.rawEndPos hval).Splits pat.copy t := by
+        apply Pos.splits_of_splits_copy
+        rw [Slice.copy_pos]
+        rw [← String.Pos.splits_cast_iff (h := ht), String.cast_pos]
+        simp only [← rawEndPos_copy]
+        exact Pos.splits_append_rawEndPos
+      simp only [Option.some.injEq]
+      rintro rfl
+      rw [pos!_eq_pos hval, hsplit.copy_sliceTo_eq]
+    · simp only [Option.some.injEq]
+      intro heq
+      rw [pos!_eq_pos hval]
+      simpa [Slice.Pos.ext_iff, Pos.Raw.ext_iff, utf8ByteSize_eq] using (congrArg String.utf8ByteSize heq).symm
+  | case2 h =>
+    simp only [startsWith_iff, not_exists] at h
+    simp only [reduceCtorEq, false_iff]
+    intro heq
+    have := h (s.sliceFrom pos).copy
+    simp [← heq, pos.splits.eq_append] at this
+
+theorem isSome_dropPrefix? {pat s : Slice} : (dropPrefix? pat s).isSome = startsWith pat s := by
+  fun_cases dropPrefix? <;> simp_all
+
+theorem lawfulForwardPatternModel {pat : Slice} (hpat : pat.isEmpty = false) :
+    LawfulForwardPatternModel pat where
+  dropPrefixOfNonempty?_eq h := rfl
+  startsWith_eq s := isSome_dropPrefix?.symm
+  dropPrefix?_eq_some_iff s := by
+    simp [ForwardPattern.dropPrefix?, dropPrefix?_eq_some_iff, isLongestMatch_iff hpat]
+
+structure PrefixProperty (b : ByteArray) (i : Nat) (hi : i < b.size) (k : Nat) : Prop where
+  le : k ≤ i
+  getElem_eq (j) (hj : j < k) : b[j] = b[i - k + 1 + j]
+
+theorem prefixProperty_iff {b : ByteArray} {i : Nat} {hi} {k : Nat} :
+    PrefixProperty b i hi k ↔ ∃ (h : k ≤ i), ∀ (j : Nat) (hj : j < k), b[j] = b[i - k + 1 + j] :=
+  ⟨fun ⟨h₁, h₂⟩ => ⟨h₁, h₂⟩, fun ⟨h₁, h₂⟩ => ⟨h₁, h₂⟩⟩
+
+theorem prefixProperty_add_one_add_one_iff {b : ByteArray} (i : Nat)
+    (hi : i + 1 < b.size) (k : Nat) :
+    PrefixProperty b (i + 1) hi (k + 1) ↔
+      ∃ (h : PrefixProperty b i (by omega) k), b[k]'(have := h.le; by omega) = b[i + 1] := by
+  refine ⟨fun ⟨hle, h⟩ => ?_, fun ⟨⟨hle, h⟩, h'⟩ => ?_⟩
+  · exact ⟨⟨by omega, fun j hj => by simp [h j (by omega)]; congr 1; omega⟩, by simp [h k (by omega)]; congr 1; omega⟩
+  · refine ⟨by omega, fun j hj => ?_⟩
+    by_cases hjk : j < k
+    · simp [h j hjk]
+      congr 1
+      omega
+    · obtain rfl : j = k := by omega
+      simp [h']
+      congr 1
+      omega
+
+theorem prefixProperty_iff_of_prefixProperty {b : ByteArray} {i : Nat} {hi : i < b.size} {k : Nat}
+    (h₀ : PrefixProperty b i hi k) {k' : Nat} :
+    PrefixProperty b (k - 1) (have := h₀.le; by omega) k' ↔ k' ≤ k - 1 ∧ PrefixProperty b i hi k' := by
+  have := h₀.le
+  refine ⟨fun ⟨hle, h⟩ => ⟨hle, ?_⟩, fun ⟨hk', ⟨hle, h⟩⟩ => ?_⟩
+  · refine ⟨by omega, fun j hj => ?_⟩
+    rw [h j hj, h₀.getElem_eq _ (by omega)]
+    congr 1
+    omega
+  · refine ⟨hk', fun j hj => ?_⟩
+    rw [h j hj]
+    conv => rhs; rw [h₀.getElem_eq _ (by omega)]
+    congr 1
+    omega
+
+instance {b i hi k} : Decidable (PrefixProperty b i hi k) :=
+  decidable_of_iff' _ prefixProperty_iff
+
+@[simp]
+theorem prefixProperty_zero {b : ByteArray} {i : Nat} {hi} : PrefixProperty b i hi 0 where
+  le := by simp
+  getElem_eq := by simp
+
+def prefixFunction (b : ByteArray) (i : Nat) (hi : i < b.size) : Nat :=
+  go i
+where go (k : Nat) : Nat :=
+  if h : PrefixProperty b i hi k then
+    k
+  else
+    have : 0 < k := Nat.pos_iff_ne_zero.2 (by rintro rfl; simp_all)
+    go (k - 1)
+
+theorem prefixFunction_eq_iff {b i hi k} :
+    prefixFunction b i hi = k ↔ PrefixProperty b i hi k ∧ ∀ k', k < k' → ¬ PrefixProperty b i hi k' := by
+  rw [prefixFunction]
+  suffices ∀ k₀,
+      (∀ k', k₀ < k' → ¬ PrefixProperty b i hi k') →
+      ∀ k, prefixFunction.go b i hi k₀ = k ↔ PrefixProperty b i hi k ∧ (∀ k', k < k' → ¬ PrefixProperty b i hi k') from
+    this _ (fun k' hk' hp => Nat.lt_irrefl _ (Nat.lt_of_le_of_lt hp.le hk')) ..
+  intro k₀ hk₀ k
+  fun_induction prefixFunction.go with
+  | case1 k' hk' =>
+    refine ⟨?_, ?_⟩
+    · rintro rfl
+      exact ⟨hk', hk₀⟩
+    · rintro ⟨h₁, h₂⟩
+      refine Nat.le_antisymm ?_ ?_ <;> exact Nat.not_lt.1 (fun hkk' => by simp_all)
+  | case2 k' hk' h₀ ih =>
+    rw [ih]
+    intro k₀ hk₀'
+    by_cases hk'k₀ : k' < k₀
+    · exact hk₀ _ hk'k₀
+    · obtain rfl : k' = k₀ := by omega
+      exact hk'
+
+theorem PrefixProperty.le_prefixFunction {b i hi k} (h : PrefixProperty b i hi k) :
+    k ≤ prefixFunction b i hi :=
+  Nat.not_lt.1 (fun hx => (prefixFunction_eq_iff.1 rfl).2 _ hx h)
+
+theorem prefixProperty_prefixFunction {b i hi} : PrefixProperty b i hi (prefixFunction b i hi) :=
+  ((prefixFunction_eq_iff).1 rfl).1
+
+theorem prefixFunction_le {b i hi} : prefixFunction b i hi ≤ i :=
+  prefixProperty_prefixFunction.le
+
+@[simp]
+theorem prefixFunction_zero {b hi} : prefixFunction b 0 hi = 0 :=
+  Nat.le_zero.1 prefixFunction_le
+
+theorem le_prefixFunction_of_prefixProperty {b i hi} {k k' : Nat} (h : k' < k)
+    (h₁ : PrefixProperty b i hi k) (h₂ : PrefixProperty b i hi k') :
+    k' ≤ prefixFunction b (k - 1) (by have := h₁.le; omega) :=
+  ((prefixProperty_iff_of_prefixProperty h₁).2 ⟨by omega, h₂⟩).le_prefixFunction
+
+structure IsComputeDistance (b : ByteArray) (i : Nat) (hi : i + 1 < b.size) (k : Nat) where
+  prefixProperty : PrefixProperty b i (by omega) k
+  not_or_ne (k') (hk' : k < k') (h₀ : k' < b.size) :
+    ¬ PrefixProperty b i (by omega) k' ∨ b[i + 1] ≠ b[k']
+  eq_zero_or : k = 0 ∨ b[i + 1] = b[k]'(have := prefixProperty.le; by omega)
+
+theorem IsComputeDistance.prefixFunction_eq {b : ByteArray} {i : Nat} {hi : i + 1 < b.size} {k : Nat}
+    (h : IsComputeDistance b i hi k) :
+    prefixFunction b (i + 1) (by omega) =
+      if b[i + 1] = b[k]'(have := h.prefixProperty.le; by omega) then k + 1 else k := by
+  split <;> rename_i h₁
+  · rw [prefixFunction_eq_iff, prefixProperty_add_one_add_one_iff]
+    refine ⟨⟨h.prefixProperty, h₁.symm⟩, fun k' hk' => ?_⟩
+    have : k' = k' - 1 + 1 := by omega
+    rw [this, prefixProperty_add_one_add_one_iff]
+    simp only [not_exists]
+    intro h''
+    have := h''.le
+    have := h.not_or_ne (k' - 1) (by omega) (by omega)
+    simp only [h'', not_true_eq_false, ne_eq, false_or] at this
+    exact Ne.symm this
+  · obtain rfl : k = 0 := by
+      obtain (h|h) := h.eq_zero_or
+      · assumption
+      · simp [h] at h₁
+    rw [prefixFunction_eq_iff]
+    refine ⟨by simp, fun k' hk' hcontr => ?_⟩
+    have : k' = k' - 1 + 1 := by omega
+    have hcle := hcontr.le
+    rw [this, prefixProperty_add_one_add_one_iff] at hcontr
+    obtain ⟨hc₁, hc₂⟩ := hcontr
+    by_cases hkk' : k' = 1
+    · cases hkk'
+      simp [hc₂] at h₁
+    · obtain (hcc|hcc) := h.not_or_ne (k' - 1) (by omega) (by omega)
+      · contradiction
+      · simp [hc₂] at hcc
+
+structure IsTable (b : ByteArray) (v : Array Nat) : Prop where
+  size_le : v.size ≤ b.size
+  eq_prefixFunction (i : Nat) (hi) : v[i]'hi = prefixFunction b i (by omega)
+
+theorem isTable_empty : IsTable ByteArray.empty #[] where
+  size_le := by simp
+  eq_prefixFunction := by simp
+
+theorem isTable_singleton {b : ByteArray} (hb : 1 ≤ b.size) : IsTable b #[0] where
+  size_le := by simp [hb]
+  eq_prefixFunction := by simp +contextual
+
+theorem IsTable.push {b : ByteArray} {v : Array Nat} (h : IsTable b v) {d : Nat}
+    (hle : v.size + 1 ≤ b.size)
+    (hd : d = prefixFunction b v.size (by omega)) :
+    IsTable b (v.push d) where
+  size_le := by simpa using hle
+  eq_prefixFunction i hi := by
+    rw [Array.getElem_push]
+    split <;> rename_i hi'
+    · rw [h.eq_prefixFunction]
+    · rw [Array.size_push] at hi
+      obtain rfl : i = v.size := by omega
+      exact hd
+
+private theorem computeDistance_correct {s : Slice} (i : Nat) (hi : i + 1 < s.copy.toByteArray.size) {patByte : UInt8}
+    (hpat : patByte = s.copy.toByteArray[i + 1])
+    (table : Array Nat) {ht} (ht' : IsTable s.copy.toByteArray table)
+    {h guess hg} (hg' : PrefixProperty s.copy.toByteArray i (by omega) guess) (ih : ∀ g', guess < g' → (hg' : g' < s.copy.toByteArray.size) →
+      ¬ PrefixProperty s.copy.toByteArray i (by omega) g' ∨ s.copy.toByteArray[i + 1] ≠ s.copy.toByteArray[g']) :
+    IsComputeDistance s.copy.toByteArray i hi
+    (buildTable.computeDistance s patByte table ht h guess hg).1 := by
+  fun_induction buildTable.computeDistance with
+  | case1 g hg hif =>
+    refine ⟨hg', ih, ?_⟩
+    simp [hpat, getUTF8Byte_eq_getUTF8Byte_copy, String.getUTF8Byte] at ⊢ hif
+    rw [eq_comm (a := s.copy.toByteArray[i + 1])]
+    exact hif
+  | case2 g hg hif htab ih₀ =>
+    apply ih₀
+    · rw [ht'.eq_prefixFunction]
+      rw [utf8ByteSize_eq_size_toByteArray_copy] at ht
+      have := prefixProperty_prefixFunction (b := s.copy.toByteArray) (i := g - 1) (hi := by omega)
+      rw [prefixProperty_iff_of_prefixProperty hg'] at this
+      exact this.2
+    · intro g' hg₀ hg'₀
+      by_cases hgg' : g < g'
+      · apply ih _ hgg'
+      · by_cases hgg₂ : g' < g
+        · refine Or.inl (fun hpp => ?_)
+          rw [ht'.eq_prefixFunction] at hg₀
+          have := le_prefixFunction_of_prefixProperty hgg₂ hg' hpp
+          omega
+        · obtain rfl : g = g' := by omega
+          refine Or.inr ?_
+          simp [hpat, getUTF8Byte_eq_getUTF8Byte_copy, String.getUTF8Byte] at hif
+          exact Ne.symm hif.2
+
+private theorem isTable_buildTableGo {s : Slice} {table : Array Nat} {ht₀ ht h}
+    (htab : IsTable s.copy.toByteArray table) :
+    IsTable s.copy.toByteArray (buildTable.go s table ht₀ ht h).toArray := by
+  fun_induction buildTable.go with
+  | case1 table ht₀ ht h h' patByte dist dist' ih =>
+    rw [utf8ByteSize_eq_size_toByteArray_copy] at h'
+    apply ih
+    apply htab.push (by omega)
+    have : IsComputeDistance s.copy.toByteArray (table.size - 1) (by omega) dist.1 := by
+      simp only [dist]
+      apply computeDistance_correct
+      · simp [patByte, (by omega : table.size - 1 + 1 = table.size),
+          getUTF8Byte_eq_getUTF8Byte_copy, String.getUTF8Byte]
+      · exact htab
+      · rw [htab.eq_prefixFunction]
+        exact prefixProperty_prefixFunction
+      · intro g' hg' hg''
+        rw [htab.eq_prefixFunction] at hg'
+        refine Or.inl (fun hcontr => ?_)
+        have := hcontr.le_prefixFunction
+        omega
+    have := this.prefixFunction_eq
+    simp only [dist']
+    simp [(by omega : table.size - 1 + 1 = table.size)] at this
+    simp [this, patByte, getUTF8Byte_eq_getUTF8Byte_copy,
+      String.getUTF8Byte]
+    simp only [eq_comm (a := s.copy.toByteArray[table.size])]
+  | case2 table ht₀ ht h h' => simpa
+
+theorem isTable_buildTable {s : Slice} : IsTable s.copy.toByteArray (buildTable s).toArray := by
+  fun_cases buildTable with
+  | case1 h =>
+    simpa [(Slice.copy_eq_empty_iff (s := s)).2 (by simp [Slice.isEmpty_eq, h])] using isTable_empty
+  | case2 h arr arr' =>
+    apply isTable_buildTableGo
+    simp [arr, arr']
+    apply isTable_singleton
+    simp [utf8ByteSize_eq] at ⊢ h
+    omega
+
+structure PartialMatch (pat s : ByteArray) (stackPos : Nat) (needlePos : Nat) : Prop where
+  hi : stackPos ≤ s.size
+  le : needlePos ≤ stackPos
+  le_size : needlePos ≤ pat.size
+  getElem_eq (j) (jh : j < needlePos) : pat[j] = s[stackPos - needlePos + j]
+
+theorem PartialMatch.zero {pat s : ByteArray} {stackPos : Nat} (h : stackPos ≤ s.size) :
+    PartialMatch pat s stackPos 0 where
+  hi := h
+  le := by simp
+  le_size := by simp
+  getElem_eq := by simp
+
+theorem PartialMatch.inc {pat s : ByteArray} {stackPos needlePos : Nat} (h₀ : PartialMatch pat s stackPos needlePos)
+    (h₁ : needlePos < pat.size) (h₂ : stackPos < s.size)
+    (h : pat[needlePos] = s[stackPos]) : PartialMatch pat s (stackPos + 1) (needlePos + 1) where
+  hi := by omega
+  le := by simp [h₀.le]
+  le_size := by omega
+  getElem_eq j hj := by
+    by_cases hj' : j < needlePos
+    · simp [h₀.getElem_eq j hj']
+      congr 1
+      omega
+    · obtain rfl : needlePos = j := by omega
+      simp [h]
+      have := h₀.le
+      congr 1
+      omega
+
+theorem PartialMatch.extract_eq {pat s : ByteArray} {stackPos : Nat} {needlePos : Nat} (h : PartialMatch pat s stackPos needlePos) :
+    s.extract (stackPos - needlePos) stackPos = pat.extract 0 needlePos := by
+  apply ByteArray.ext_getElem
+  · simp [h.le_size, h.hi]
+    have := h.le
+    omega
+  · intro i hi hi'
+    simp [ByteArray.getElem_extract, h.getElem_eq i (by simp_all; omega)]
+
+theorem PartialMatch.extract_eq_all {pat s : ByteArray} {stackPos needlePos : Nat} (h : PartialMatch pat s stackPos needlePos) (h' : needlePos = pat.size) :
+    s.extract (stackPos - needlePos) stackPos = pat := by
+  rw [h.extract_eq, h', ByteArray.extract_zero_size]
+
+theorem PartialMatch.partialMatch_of_prefixFunction_eq {pat s : ByteArray} {stackPos needlePos : Nat}
+    (h : PartialMatch pat s stackPos needlePos) (h' : 0 < needlePos) {k : Nat} {hki} (hk : prefixFunction pat (needlePos - 1) hki = k) :
+    PartialMatch pat s stackPos k := by
+  cases hk
+  obtain ⟨h₁, h₂⟩ := prefixProperty_prefixFunction (hi := hki)
+  refine ⟨?_, ?_, ?_, ?_⟩
+  · exact h.hi
+  · have := h.le
+    omega
+  · omega
+  · intro j hj
+    have := h.getElem_eq
+    have : stackPos - prefixFunction pat (needlePos - 1) hki + j =
+        stackPos - needlePos + (needlePos - 1 - prefixFunction pat (needlePos - 1) hki + 1 + j) := by
+      have := h.le
+      omega
+    simp only [this]
+    rw [← h.getElem_eq]
+    · rw [h₂ _ hj]
+    · omega
+
+-- theorem PartialMatch.not_matchesAt_of_prefixFunction_eq {pat s : ByteArray} {stackPos needlePos : Nat}
+--     (h : PartialMatch pat s stackPos needlePos) (h' : 0 < needlePos) {h : Nat} {hki} (hk : prefixFunction pat (needlePos - 1) hki = k) :
+--     False := sorry
+
+structure Invariants (pat s : Slice) (stackPos needlePos : String.Pos.Raw) : Prop where
+  isEmpty_eq_false : pat.isEmpty = false
+  partialMatch : PartialMatch pat.copy.toByteArray s.copy.toByteArray stackPos.byteIdx needlePos.byteIdx
+  isValid : (stackPos.unoffsetBy needlePos).IsValidForSlice s
+
+theorem Invariants.start (pat s : Slice) (h : pat.isEmpty = false) : Invariants pat s s.startPos.offset pat.startPos.offset where
+  isEmpty_eq_false := h
+  partialMatch := .zero (by simp)
+  isValid := by simp [Pos.Raw.unoffsetBy]
+
+theorem Invariants.offset {pat s : Slice} (h : pat.isEmpty = false) (p : s.Pos) : Invariants pat s p.offset pat.startPos.offset where
+  isEmpty_eq_false := h
+  partialMatch := .zero
+    (by rw [← utf8ByteSize_eq_size_toByteArray_copy, ← byteIdx_rawEndPos, ← Pos.Raw.le_iff]; simp)
+  isValid := by simp
+
+theorem Invariants.inc {pat s : Slice} {stackPos needlePos : String.Pos.Raw} (h₀ : Invariants pat s stackPos needlePos)
+    (h₁ h₂)
+    (h : pat.getUTF8Byte needlePos h₁ = s.getUTF8Byte stackPos h₂) : Invariants pat s stackPos.inc needlePos.inc where
+  isEmpty_eq_false := h₀.isEmpty_eq_false
+  partialMatch := h₀.partialMatch.inc (by simpa using h₁) (by simpa using h₂) (by simpa [getUTF8Byte_eq_getUTF8Byte_copy] using h)
+  isValid := by simpa using h₀.isValid
+
+theorem Invariants.of_prefixFunction_eq {pat s : Slice} {stackPos needlePos : String.Pos.Raw} (hst : stackPos < s.rawEndPos) (h : Invariants pat s stackPos needlePos)
+    (h' : 0 < needlePos) {k : Nat} {hki} (hk : prefixFunction pat.copy.toByteArray (needlePos.byteIdx - 1) hki = k) (hk₀ : 0 < k) :
+    Invariants pat s stackPos ⟨k⟩ := by
+  refine ⟨h.isEmpty_eq_false, h.partialMatch.partialMatch_of_prefixFunction_eq h' hk, ?_⟩
+  rw [Pos.Raw.isValidForSlice_iff_isUTF8FirstByte]
+  refine Or.inr ⟨?_, ?_⟩
+  · simp [Pos.Raw.lt_iff] at ⊢ hst
+    omega
+  · have := (h.partialMatch.partialMatch_of_prefixFunction_eq h' hk).getElem_eq 0 hk₀
+    simp at this
+    rw [getUTF8Byte_eq_getUTF8Byte_copy, String.getUTF8Byte]
+    simp
+    rw [← this]
+    exact isUTF8FirstByte_getUTF8Byte_zero
+
+theorem Invariants.prefixProperty_of_matchesAt {pat s : Slice} {stackPos needlePos : String.Pos.Raw}
+    (h : Invariants pat s stackPos needlePos) (h' : 0 < needlePos.byteIdx) (pos : s.Pos)
+    (hp' : stackPos.byteIdx - pos.offset.byteIdx ≤ needlePos.byteIdx - 1)
+    (hm : MatchesAt pat pos) :
+    PrefixProperty pat.copy.toByteArray
+      (needlePos.byteIdx - 1) (by have := h.partialMatch.le_size; omega) (stackPos.byteIdx - pos.offset.byteIdx) :=by
+  refine ⟨by omega, fun j hj => ?_⟩
+  have := h.partialMatch.getElem_eq
+  rw [getElem_eq_of_matchesAt h.isEmpty_eq_false hm, this]
+  · congr 1
+    have := h.partialMatch.le
+    omega
+  · omega
+
+theorem Invariants.not_matchesAt_of_prefixFunction_eq {pat s : Slice} {stackPos needlePos : String.Pos.Raw}
+    (h : Invariants pat s stackPos needlePos)
+    (h' : 0 < needlePos) {k : Nat} {hki} (hk : prefixFunction pat.copy.toByteArray (needlePos.byteIdx - 1) hki = k)
+    (p : s.Pos) (hp₁ : stackPos.unoffsetBy needlePos ≤ p.offset) (hp₂ : p.offset < stackPos.unoffsetBy ⟨k⟩)
+    {h₁ h₂}
+    (hmism : s.getUTF8Byte stackPos h₁ ≠ pat.getUTF8Byte needlePos h₂) :
+    ¬ MatchesAt pat p := by
+  by_cases hcas : stackPos.byteIdx - p.offset.byteIdx ≤ needlePos.byteIdx - 1
+  · intro hcontr
+    have := h.prefixProperty_of_matchesAt h' _ hcas hcontr
+    have := this.le_prefixFunction
+    rw [hk] at this
+    simp [Pos.Raw.lt_iff] at hp₂
+    omega
+  · obtain rfl : stackPos = needlePos.offsetBy p.offset := by
+      simp [Pos.Raw.le_iff, Pos.Raw.ext_iff] at hp₁ ⊢
+      omega
+    exact not_matchesAt_of_getUTF8Byte_ne h.isEmpty_eq_false _ hmism
+
+section
+
+variable {pat s : Slice} {stackPos needlePos : String.Pos.Raw}
+
+theorem Invariants.extract_eq (h : Invariants pat s stackPos needlePos) :
+    s.copy.toByteArray.extract (stackPos.unoffsetBy needlePos).byteIdx stackPos.byteIdx = pat.copy.toByteArray.extract 0 needlePos.byteIdx :=
+  h.partialMatch.extract_eq
+
+theorem Invariants.extract_eq_all (h : Invariants pat s stackPos needlePos) (h' : needlePos = pat.rawEndPos) :
+    s.copy.toByteArray.extract (stackPos.unoffsetBy needlePos).byteIdx stackPos.byteIdx = pat.copy.toByteArray :=
+  h.partialMatch.extract_eq_all (by simpa [Pos.Raw.ext_iff] using h')
+
+theorem Invariants.isValidUTF8 (h : Invariants pat s stackPos needlePos) (h' : needlePos = pat.rawEndPos) :
+    (s.copy.toByteArray.extract (stackPos.unoffsetBy needlePos).byteIdx stackPos.byteIdx).IsValidUTF8 := by
+  rw [h.extract_eq_all h']
+  exact pat.copy.isValidUTF8
+
+theorem Invariants.stackPos_le_rawEndPos (h : Invariants pat s stackPos needlePos) :
+    stackPos ≤ s.rawEndPos := by
+  simpa [Pos.Raw.le_iff] using h.partialMatch.hi
+
+theorem Invariants.isValidForSlice_stackPos (h : Invariants pat s stackPos needlePos) (h' : needlePos = pat.rawEndPos) :
+    stackPos.IsValidForSlice s := by
+  obtain (hx|hx) := (Pos.Raw.isValidUTF8_extract_iff _ _ (by simp) (by simpa using h.stackPos_le_rawEndPos)).1 (h.isValidUTF8 h')
+  · rw [← hx]
+    exact h.isValid
+  · exact Pos.Raw.isValid_copy_iff.1 hx.2
+
+theorem Invariants.isValidForSlice_stackPos_zero (h : Invariants pat s stackPos needlePos) (h' : needlePos.byteIdx = 0) :
+    stackPos.IsValidForSlice s := by
+  suffices stackPos.unoffsetBy needlePos = stackPos by simpa [this] using h.isValid
+  simp [Pos.Raw.ext_iff, h']
+
+def Invariants.base (h : Invariants pat s stackPos needlePos) : s.Pos :=
+  s.pos _ h.isValid
+
+def Invariants.stackValidPos (h : Invariants pat s stackPos needlePos) (h' : needlePos = pat.rawEndPos) : s.Pos :=
+  s.pos _ (h.isValidForSlice_stackPos h')
+
+theorem Invariants.isLongestMatchAt (h : Invariants pat s stackPos needlePos) (h' : needlePos = pat.rawEndPos) :
+    IsLongestMatchAt pat h.base (h.stackValidPos h') := by
+  rw [isLongestMatchAt_iff_extract h.isEmpty_eq_false, ← h.extract_eq_all h']
+  simp [base, stackValidPos]
+
+end
+
+
+theorem Invariants.base_start {pat s : Slice} (h : pat.isEmpty = false) : (Invariants.start pat s h).base = s.startPos :=
+  (rfl)
+
+theorem Invariants.isValidSearchFrom_toList {pat s : Slice} {stackPos needlePos : String.Pos.Raw}
+    (hpat : pat.isEmpty = false)
+    (it : Std.Iter (α := ForwardSliceSearcher s) (SearchStep s))
+    (h : Invariants pat s stackPos needlePos)
+    {table ht hn}
+    (heq : it = Std.Iter.mk (.proper pat table ht stackPos needlePos hn)) {p : s.Pos} (hp : p = h.base) :
+    IsValidSearchFrom pat p it.toList := by
+  induction it using Std.Iter.inductSteps generalizing p stackPos needlePos with | step it ihy ihs
+  cases heq
+  cases hp
+  rw [Std.Iter.toList_eq_match_step]
+  generalize hit' : (Std.Iter.mk (α := ForwardSliceSearcher s) (.proper pat table ht stackPos needlePos hn)).step = it'
+
+  have hit'' := congrArg Subtype.val hit'
+  have plausible := it'.property
+  simp only [Std.Iter.step_eq, ne_eq, Std.Iter.toIterM] at hit''
+  split at hit'' <;> rename_i h₁
+  · split at hit'' <;> rename_i h₂
+    · split at hit'' <;> rename_i h₃
+      · have hinc := h.inc _ _ h₂.symm
+        simp only [Id.run_pure, Std.Shrink.inflate_deflate,
+          Std.IterM.Step.toPure_yield, Std.PlausibleIterStep.yield] at hit''
+        rw [s.pos!_eq_pos hinc.isValid, s.pos!_eq_pos (hinc.isValidForSlice_stackPos h₃)] at hit''
+        simp [← hit''] at ⊢ plausible
+        apply IsValidSearchFrom.matched_of_eq
+        · apply ihy plausible _ rfl rfl
+          exact ⟨hpat, .zero (by simpa [Pos.Raw.le_iff, Pos.Raw.lt_iff]),
+            by simpa using hinc.isValidForSlice_stackPos h₃⟩
+        · simpa [Invariants.base] using hinc.isLongestMatchAt h₃
+        · simp [Invariants.base]
+      · have hinc := h.inc _ _ h₂.symm
+        simp only [Id.run_pure, Std.Shrink.inflate_deflate, Std.IterM.Step.toPure_skip,
+          Std.PlausibleIterStep.skip] at hit''
+        simp [← hit''] at ⊢ plausible
+        exact ihs plausible hinc rfl (by simp [Invariants.base])
+    · split at hit'' <;> rename_i h₃
+      · simp only [Id.run_pure, Std.Shrink.inflate_deflate, Std.IterM.Step.toPure_yield,
+          Std.PlausibleIterStep.yield] at hit''
+        obtain rfl : needlePos = 0 := by simpa [Pos.Raw.ext_iff]
+        rw [pos!_eq_pos (h.isValidForSlice_stackPos_zero h₃)] at hit''
+        simp [← hit''] at ⊢ plausible
+        apply IsValidSearchFrom.mismatched_of_eq
+        · exact ihy plausible (.offset hpat _) rfl rfl
+        · simp only [base, Pos.lt_iff, offset_pos]
+          exact Pos.Raw.lt_of_le_of_lt Pos.Raw.unoffsetBy_le_self lt_offset_posGT
+        · intro p hp₁ hp₂
+          simp [base] at hp₁
+          rw [posGT_eq_next (h.isValidForSlice_stackPos_zero h₃),
+            Pos.lt_next_iff_le] at hp₂
+          obtain rfl : p = s.pos stackPos (h.isValidForSlice_stackPos_zero h₃) :=
+            Std.le_antisymm hp₂ hp₁
+          exact not_matchesAt_of_getUTF8Byte_ne hpat 0 h₂
+        · simp [base]
+      · simp [Pos.Raw.lt_iff] at hn
+        have hxx : needlePos.byteIdx - 1 < pat.utf8ByteSize := by omega
+        have hxx' : needlePos.byteIdx - 1 < pat.copy.toByteArray.size := by
+          rw [← utf8ByteSize_eq_size_toByteArray_copy]; omega
+        have htt : table[needlePos.byteIdx - 1] = prefixFunction pat.copy.toByteArray (needlePos.byteIdx - 1) hxx' := by
+          cases ht
+          rw [← Vector.getElem_toArray, isTable_buildTable.eq_prefixFunction]
+          simpa
+        split at hit'' <;> rename_i h₄
+        · simp only [Id.run_pure, Std.Shrink.inflate_deflate, Std.IterM.Step.toPure_yield,
+            Std.PlausibleIterStep.yield] at hit''
+          rw [pos!_eq_pos h.isValid] at hit''
+          simp [← hit''] at ⊢ plausible
+          apply IsValidSearchFrom.mismatched_of_eq
+          · exact ihy plausible (.offset hpat _) rfl rfl
+          · simp [base]
+            have := h.partialMatch.le
+            simp [Pos.Raw.lt_iff]
+            omega
+          · intro p hp₁ hp₂
+            simp [base, Pos.le_iff] at hp₁
+            rw [lt_posGE_iff] at hp₂
+            exact h.not_matchesAt_of_prefixFunction_eq (by simp [Pos.Raw.lt_iff]; omega) htt.symm
+              _ hp₁ (by simpa [h₄]) h₂
+          · simp [base]
+        · simp only [Id.run_pure, Std.Shrink.inflate_deflate, Std.IterM.Step.toPure_yield,
+            Std.PlausibleIterStep.yield] at hit''
+          have hinv := h.of_prefixFunction_eq h₁ (by simp [Pos.Raw.lt_iff]; omega) htt.symm (by omega)
+          rw [pos!_eq_pos h.isValid, pos!_eq_pos hinv.isValid] at hit''
+          simp [← hit''] at ⊢ plausible
+          apply IsValidSearchFrom.mismatched_of_eq
+          · exact ihy plausible hinv rfl rfl
+          · simp [base, Pos.lt_iff, Pos.Raw.lt_iff]
+            have := h.partialMatch.le
+            suffices table[needlePos.byteIdx - 1] < needlePos.byteIdx by omega
+            rw [htt]
+            refine Std.lt_of_le_of_lt (prefixProperty_prefixFunction).le (by omega)
+          · intro p hp₁ hp₂
+            simp [base, Pos.le_iff] at hp₁
+            simp [Pos.lt_iff] at hp₂
+            exact h.not_matchesAt_of_prefixFunction_eq (by simp [Pos.Raw.lt_iff]; omega) htt.symm
+              _ hp₁ hp₂ h₂
+          · simp [base]
+  · obtain rfl : stackPos = s.rawEndPos := by
+      have := h.partialMatch.hi
+      rw [← utf8ByteSize_eq_size_toByteArray_copy, ← byteIdx_rawEndPos, ← Pos.Raw.le_iff] at this
+      rw [Std.not_lt] at h₁
+      exact Std.le_antisymm this h₁
+    split at hit'' <;> rename_i h₂
+    · simp only [Id.run_pure, Std.Shrink.inflate_deflate, Std.IterM.Step.toPure_yield,
+        Std.PlausibleIterStep.yield] at hit''
+      rw [pos!_eq_pos h.isValid] at hit''
+      simp [← hit''] at ⊢ plausible
+      apply IsValidSearchFrom.mismatched_of_eq
+      · rw [Std.Iter.toList_eq_match_step, Std.Iter.step_eq]
+        simpa [Std.Iter.toIterM] using IsValidSearchFrom.endPos
+      · have := h.partialMatch.le
+        have := h.partialMatch.hi
+        rw [← utf8ByteSize_eq_size_toByteArray_copy] at this
+        simp [base, Pos.lt_iff, Pos.Raw.lt_iff] at ⊢ h₁ h₂
+        omega
+      · intro pos hp₁ hp₂ hcontr
+        have := le_of_matchesAt hpat hcontr
+        have := h.partialMatch.le_size
+        rw [← utf8ByteSize_eq_size_toByteArray_copy] at this
+        simp [base, Pos.Raw.le_iff, Pos.le_iff, Pos.Raw.lt_iff] at hp₁ h₂ hn
+        omega
+      · simp [base]
+    · obtain rfl : needlePos = 0 := by
+        simpa [Pos.Raw.ext_iff, Pos.Raw.lt_iff] using h₂
+      simpa [← hit'', base] using IsValidSearchFrom.endPos
+
+
+theorem lawfulToForwardSearcherModel {pat : Slice} (hpat : pat.isEmpty = false) :
+    LawfulToForwardSearcherModel pat where
+  isValidSearchFrom_toList s := by
+    simp only [ToForwardSearcher.toSearcher]
+    rw [iter, dif_neg (by simpa [isEmpty_eq] using hpat)]
+    rw (occs := [1]) [← Invariants.base_start hpat]
+    apply Invariants.isValidSearchFrom_toList hpat _ _ rfl rfl
+
+end ForwardSliceSearcher
+
+end Pattern
+
+end String.Slice
