src/Init/Data/String/Positions.lean
@@ -1,0 +1,144 @@
+/-
+Copyright (c) 2025 Lean FRO, LLC. All rights reserved.
+Released under Apache 2.0 license as described in the file LICENSE.
+Authors: Henrik Böving, Markus Himmel
+-/
+module
+
+prelude
+public import Init.Data.String.Basic
+public import Init.Data.Iterators.Consumers.Monadic.Loop
+public import Init.Data.String.Iter
+import Init.Data.Iterators.Combinators.FilterMap
+import Init.Data.String.Termination
+
+set_option doc.verso true
+
+public section
+
+namespace String.Slice
+
+structure PosIterator (s : Slice) where
+  currPos : s.Pos
+deriving Inhabited
+
+set_option doc.verso false
+/--
+Creates an iterator over all valid positions within {name}`s`.
+Examples
+ * {lean}`("abc".toSlice.positions.map (fun ⟨p, h⟩ => p.get h) |>.toList) = ['a', 'b', 'c']`
+ * {lean}`("abc".toSlice.positions.map (·.val.offset.byteIdx) |>.toList) = [0, 1, 2]`
+ * {lean}`("ab∀c".toSlice.positions.map (fun ⟨p, h⟩ => p.get h) |>.toList) = ['a', 'b', '∀', 'c']`
+ * {lean}`("ab∀c".toSlice.positions.map (·.val.offset.byteIdx) |>.toList) = [0, 1, 2, 5]`
+-/
+def positions (s : Slice) : Std.Iter (α := PosIterator s) { p : s.Pos // p ≠ s.endPos } :=
+  { internalState := { currPos := s.startPos }}
+
+set_option doc.verso true
+
+namespace PosIterator
+
+instance : Std.Iterator (PosIterator s) Id { p : s.Pos // p ≠ s.endPos } where
+  IsPlausibleStep it
+    | .yield it' out =>
+      ∃ h : it.internalState.currPos ≠ s.endPos,
+        it'.internalState.currPos = it.internalState.currPos.next h ∧
+        it.internalState.currPos = out
+    | .skip _ => False
+    | .done => it.internalState.currPos = s.endPos
+  step := fun ⟨⟨currPos⟩⟩ =>
+    if h : currPos = s.endPos then
+      pure (.deflate ⟨.done, by simp [h]⟩)
+    else
+      pure (.deflate ⟨.yield ⟨⟨currPos.next h⟩⟩ ⟨currPos, h⟩, by simp [h]⟩)
+
+private def finitenessRelation :
+    Std.Iterators.FinitenessRelation (PosIterator s) Id where
+  Rel := InvImage WellFoundedRelation.rel (fun it => it.internalState.currPos)
+  wf := InvImage.wf _ WellFoundedRelation.wf
+  subrelation {it it'} h := by
+    simp_wf
+    obtain ⟨step, h, h'⟩ := h
+    cases step
+    · cases h
+      obtain ⟨_, h2, _⟩ := h'
+      simp [h2]
+    · cases h'
+    · cases h
+
+@[no_expose]
+instance : Std.Iterators.Finite (PosIterator s) Id :=
+  .of_finitenessRelation finitenessRelation
+
+instance : Std.IteratorLoop (PosIterator s) Id Id :=
+  .defaultImplementation
+
+docs_to_verso positions
+
+end PosIterator
+
+structure RevPosIterator (s : Slice) where
+  currPos : s.Pos
+deriving Inhabited
+
+set_option doc.verso false
+/--
+Creates an iterator over all valid positions within {name}`s`, starting from the last valid
+position and iterating towards the first one.
+Examples
+ * {lean}`("abc".toSlice.revPositions.map (fun ⟨p, h⟩ => p.get h) |>.toList) = ['c', 'b', 'a']`
+ * {lean}`("abc".toSlice.revPositions.map (·.val.offset.byteIdx) |>.toList) = [2, 1, 0]`
+ * {lean}`("ab∀c".toSlice.revPositions.map (fun ⟨p, h⟩ => p.get h) |>.toList) = ['c', '∀', 'b', 'a']`
+ * {lean}`("ab∀c".toSlice.revPositions.map (·.val.offset.byteIdx) |>.toList) = [5, 2, 1, 0]`
+-/
+def revPositions (s : Slice) : Std.Iter (α := RevPosIterator s) { p : s.Pos // p ≠ s.endPos } :=
+  { internalState := { currPos := s.endPos }}
+
+set_option doc.verso true
+
+namespace RevPosIterator
+
+instance [Pure m] :
+    Std.Iterator (RevPosIterator s) m { p : s.Pos // p ≠ s.endPos } where
+  IsPlausibleStep it
+    | .yield it' out =>
+      ∃ h : it.internalState.currPos ≠ s.startPos,
+        it'.internalState.currPos = it.internalState.currPos.prev h ∧
+        it.internalState.currPos.prev h = out
+    | .skip _ => False
+    | .done => it.internalState.currPos = s.startPos
+  step := fun ⟨⟨currPos⟩⟩ =>
+    if h : currPos = s.startPos then
+      pure (.deflate ⟨.done, by simp [h]⟩)
+    else
+      let prevPos := currPos.prev h
+      pure (.deflate ⟨.yield ⟨⟨prevPos⟩⟩ ⟨prevPos, Pos.prev_ne_endPos⟩, by simp [h, prevPos]⟩)
+
+private def finitenessRelation [Pure m] :
+    Std.Iterators.FinitenessRelation (RevPosIterator s) m where
+  Rel := InvImage WellFoundedRelation.rel
+      (fun it => it.internalState.currPos.down)
+  wf := InvImage.wf _ WellFoundedRelation.wf
+  subrelation {it it'} h := by
+    simp_wf
+    obtain ⟨step, h, h'⟩ := h
+    cases step
+    · cases h
+      obtain ⟨h1, h2, _⟩ := h'
+      simp [h2]
+    · cases h'
+    · cases h
+
+@[no_expose]
+instance [Pure m] : Std.Iterators.Finite (RevPosIterator s) m :=
+  .of_finitenessRelation finitenessRelation
+
+instance [Monad m] [Monad n] : Std.IteratorLoop (RevPosIterator s) m n :=
+  .defaultImplementation
+
+docs_to_verso revPositions
+
+end RevPosIterator
+
+
+end String.Slice
